Make [has_next] and [has_prev] accept nullable nodes

ind/DoublyLinkedListIface.fst
@@ -528,6 +528,8 @@ let rec _lemma_length_g_node_vals (h0:HS.mem) (l:list (node 'a)) :
 
 let has_next d n =
   let h0 = HST.get () in
+  if is_null_node n then false else
+  let n = coerce_non_null n in
   DLL.lemma_dll_links_contained h0 (d@h0) (as_list h0 d `L.index_of` n);
   L.lemma_unsnoc_is_last (as_list h0 d);
   let y = not (B.is_null (!*n).DLL.flink) in
@@ -543,6 +545,8 @@ let has_next d n =
 
 let has_prev d n =
   let h0 = HST.get () in
+  if is_null_node n then false else
+  let n = coerce_non_null n in
   DLL.lemma_dll_links_contained h0 (d@h0) (as_list h0 d `L.index_of` n);
   L.lemma_unsnoc_is_last (as_list h0 d);
   let y = not (B.is_null (!*n).DLL.blink) in
